cogent/isa/Cogent.thy
@@ -1021,6 +1021,7 @@ lemma kinding_simps:
   "\<And>K ts k.     K \<turnstile> (TSum ts) :\<kappa> k        \<longleftrightarrow> (K \<turnstile>* ts :\<kappa>v k) \<and> distinct (map fst ts)"
   "\<And>K ta tb k.  K \<turnstile> (TProduct ta tb) :\<kappa> k \<longleftrightarrow> (K \<turnstile> ta :\<kappa> k) \<and> (K \<turnstile> tb :\<kappa> k)"
   "\<And>K ts s k.   K \<turnstile> (TRecord ts s) :\<kappa> k   \<longleftrightarrow> (K \<turnstile>* ts :\<kappa>r k) \<and> k \<subseteq> sigil_kind s \<and> distinct (map fst ts)"
+  "\<And>K t n s k.  K \<turnstile> (TArray t n s) :\<kappa> k   \<longleftrightarrow> (K \<turnstile> t :\<kappa> k) \<and> k \<subseteq> sigil_kind s "
   "\<And>K k.        K \<turnstile> TUnit :\<kappa> k            \<longleftrightarrow> k \<subseteq> UNIV"
   by (auto simp add: kinding_defs list_all_iff)
 
